code/ecdsap256/Hacl.Impl.P256.LowLevel.PrimeSpecific.fsti
@@ -14,8 +14,8 @@ open FStar.Mul
 
 
 inline_for_extraction
-let prime256_buffer: x: glbuffer uint64 4ul {witnessed #uint64 #(size 4) x (Lib.Sequence.of_list p256_prime_list) /\ recallable x /\ felem_seq_as_nat (Lib.Sequence.of_list (p256_prime_list)) == prime256} = 
-  assert_norm (felem_seq_as_nat (Lib.Sequence.of_list (p256_prime_list)) == prime256);
+let prime256_buffer: x: glbuffer uint64 4ul {witnessed #uint64 #(size 4) x (Lib.Sequence.of_list p256_prime_list) /\ recallable x /\ felem_seq_as_nat P256 (Lib.Sequence.of_list (p256_prime_list)) == prime256} = 
+  assert_norm (felem_seq_as_nat P256 (Lib.Sequence.of_list (p256_prime_list)) == prime256);
   createL_global p256_prime_list
 
 val reduction_prime_2prime_with_carry: #c: curve -> x: widefelem c -> result: felem c -> 
